# Point 1.1 - Simplify expressions

## Expression a)

$$              
    \begin{matrix}
        expr &      = & 3x^2 + 2x^2     \\ 
        &           = & \bm{ 5x^2 }
    \end{matrix}
$$

## Expression b)

$$
    \begin{matrix}
        expr &      = & (3x)^2 + (2x)^2         \\
        &           = & 3x * 3x + 2x * 2x       \\
        &           = & 9x^2 + 4x^2             \\ 
        &           = & \bm{ 13x^2 }
    \end{matrix}
$$

## Expression c)

$$              
    \begin{matrix}
        expr &      = & x^4 + 3x^3 + x^2 - x - (x^3 - 2 x^2 - x)    \\
        &           = & x^4 + 3x^3 + x^2 - x - x^3 + 2 x^2 + x      \\ 
        &           = & \bm{ x^4 + 2x^3 + 3x^2 }
    \end{matrix}
$$
